genmakefile: account for *StaticAssertions.c

src/3d/Deps.fst
@@ -13,6 +13,7 @@ type dep_graph' = list edge
 type dep_graph = {
   graph: dep_graph';
   modules_with_entrypoint: list string;
+  modules_with_static_assertions: list string;
 }
 
 let all_edges_from (g:dep_graph') (node:string) : Tot (list edge) =
@@ -50,11 +51,19 @@ let rec topsort_aux (g:dep_graph') (root:string) (acc:list string & list string)
 let topsort (g:dep_graph') (root:string) : ML (list string) =
   topsort_aux g root ([root], []) |> snd |> List.rev
 
-let scan_deps (fn:string) : ML (bool & list string) =
+noeq
+type scan_deps_t = {
+  sd_deps: list string;
+  sd_has_entrypoint: bool;
+  sd_has_static_assertions: bool;
+}
+
+let scan_deps (fn:string) : ML scan_deps_t =
   let dirname = OS.dirname fn in
-  let decls, __refinement = ParserDriver.parse fn in  //AR: TODO: look into refinement too?
+  let decls, refinement = ParserDriver.parse fn in  //AR: TODO: look into refinement too?
 
   let has_entrypoint = List.Tot.existsb is_entrypoint decls in
+  let has_static_assertions = Some? refinement in
 
   let abbrevs = H.create 10 in
 
@@ -162,7 +171,11 @@ let scan_deps (fn:string) : ML (bool & list string) =
       (deps_of_params params)@
       (deps_of_switch_case sc) in
 
-  (has_entrypoint, List.collect deps_of_decl decls)
+  {
+    sd_deps = List.collect deps_of_decl decls;
+    sd_has_entrypoint = has_entrypoint;
+    sd_has_static_assertions = has_static_assertions;
+  }
 
 let rec build_dep_graph_aux (dirname:string) (mname:string) (acc:dep_graph & list string)
   : ML (dep_graph & list string) =  //seen
@@ -170,7 +183,9 @@ let rec build_dep_graph_aux (dirname:string) (mname:string) (acc:dep_graph & lis
   let g, seen = acc in
   if List.mem mname seen then acc
   else
-    let (has_entrypoint, deps) = scan_deps (Options.get_file_name (OS.concat dirname mname)) in
+    let {sd_has_entrypoint = has_entrypoint; sd_deps = deps; sd_has_static_assertions = has_static_assertions} =
+      scan_deps (Options.get_file_name (OS.concat dirname mname))
+    in
     let edges = List.fold_left (fun edges dep ->
       if List.mem (mname, dep) edges
       then edges
@@ -178,6 +193,7 @@ let rec build_dep_graph_aux (dirname:string) (mname:string) (acc:dep_graph & lis
     let g' = {
       graph = g.graph @ edges;
       modules_with_entrypoint = (if has_entrypoint then mname :: g.modules_with_entrypoint else g.modules_with_entrypoint);
+      modules_with_static_assertions = (if has_static_assertions then mname :: g.modules_with_static_assertions else g.modules_with_static_assertions);
     }
     in
     List.fold_left (fun acc dep -> build_dep_graph_aux dirname dep acc)
@@ -187,6 +203,7 @@ let build_dep_graph_from_list files =
   let g0 = {
     graph = [];
     modules_with_entrypoint = [];
+    modules_with_static_assertions = [];
   }
   in
   List.fold_left (fun acc fn -> build_dep_graph_aux (OS.dirname fn) (Options.get_module_name fn) acc) (g0, []) files
@@ -205,3 +222,5 @@ let collect_and_sort_dependencies_from_graph (g: dep_graph) (files:list string) 
   |> List.map filename_of
 
 let has_entrypoint g m = List.Tot.mem m g.modules_with_entrypoint
+
+let has_static_assertions g m = List.Tot.mem m g.modules_with_static_assertions
