src/3d/Deps.fsti
@@ -14,3 +14,5 @@ let collect_and_sort_dependencies (files:list string) : ML (list string) =
   collect_and_sort_dependencies_from_graph (build_dep_graph_from_list files) files
 
 val has_entrypoint (g: dep_graph) (modul: string) : Tot bool
+
+val has_static_assertions (g: dep_graph) (modul: string) : Tot bool
